src/Spec/Machine.v
@@ -5,20 +5,21 @@ Require Import riscv.Spec.Decode.
 
 
 Inductive AccessType: Type := Instr | Load | Store.
+Inductive SourceType: Type := VirtualMemory | Fetch | Execute.
 
 Class RiscvProgram{M}{t}`{Monad M}`{MachineWidth t} := mkRiscvProgram {
   getRegister: Register -> M t;
   setRegister: Register -> t -> M unit;
 
-  loadByte: t -> M w8;
-  loadHalf: t -> M w16;
-  loadWord: t -> M w32;
-  loadDouble: t -> M w64;
+  loadByte   : SourceType -> t -> M w8;
+  loadHalf   : SourceType -> t -> M w16;
+  loadWord   : SourceType -> t -> M w32;
+  loadDouble : SourceType -> t -> M w64;
 
-  storeByte: t -> w8 -> M unit;
-  storeHalf: t -> w16 -> M unit;
-  storeWord: t -> w32 -> M unit;
-  storeDouble: t -> w64 -> M unit;
+  storeByte   : SourceType -> t -> w8 -> M unit;
+  storeHalf   : SourceType -> t -> w16 -> M unit;
+  storeWord   : SourceType -> t -> w32 -> M unit;
+  storeDouble : SourceType -> t -> w64 -> M unit;
 
   getPC: M t;
   setPC: t -> M unit;
@@ -29,11 +30,11 @@ Class RiscvProgram{M}{t}`{Monad M}`{MachineWidth t} := mkRiscvProgram {
   isPhysicalMemAddr: t -> M bool;
      not needed at the moment because we expose state record *)
 
-  raiseException{A: Type}(isInterrupt: t)(exceptionCode: t): M A;
+  raiseExceptionWithInfo{A: Type}(isInterrupt: t)(exceptionCode: t)(info: t): M A;
 }.
 
 
-Class RiscvState`{MP: RiscvProgram} := mkRiscvState {
+Class RiscvMachine`{MP: RiscvProgram} := mkRiscvMachine {
   (* checks that addr is aligned, and translates the (possibly virtual) addr to a physical
      address, raising an exception if the address is invalid *)
   translate(accessType: AccessType)(alignment: t)(addr: t): M t;
@@ -54,6 +55,10 @@ Section Riscv.
   Local Open Scope alu_scope.
   Local Open Scope Z_scope.
 
+  Definition raiseException{A: Type}{MP: RiscvProgram}
+             (isInterrupt: t)(exceptionCode: t): M A :=
+    raiseExceptionWithInfo isInterrupt exceptionCode (ZToReg 0).
+
   (* in a system with virtual memory, this would also do the translation, but in our
      case, we only verify the alignment *)
   Definition translate_with_alignment_check{MP: RiscvProgram}
@@ -62,7 +67,7 @@ Section Riscv.
     then raiseException (ZToReg 0) (ZToReg 4)
     else Return addr.
 
-  Instance DefaultRiscvState{MP: RiscvProgram}: RiscvState := {|
+  Instance DefaultRiscvState{MP: RiscvProgram}: RiscvMachine := {|
     (* riscv does allow misaligned memory access (but might emulate them in software),
        so for the compiler-facing side, we don't do alignment checks, but might add
        another riscv machine layer below to emulate turn misaligned accesses into two
@@ -76,7 +81,7 @@ Definition Register0: Register := 0%Z.
 
 Arguments RiscvProgram: clear implicits.
 Arguments RiscvProgram (M) (t) {_} {_}.
-Arguments RiscvState: clear implicits.
-Arguments RiscvState (M) (t) {_} {_} {_}.
+Arguments RiscvMachine: clear implicits.
+Arguments RiscvMachine (M) (t) {_} {_} {_}.
 
 Existing Instance DefaultRiscvState.
