convert-hs-to-coq/Execute_preamble.v
@@ -1,3 +1,4 @@
 Require Import Coq.ZArith.BinInt.
 Local Open Scope Z.
+Require Import riscv.Utility.Utility.
 Local Open Scope alu_scope.
