src/Spec/ExecuteI.v
@@ -14,6 +14,7 @@ Require Coq.Program.Wf.
 
 Require Import Coq.ZArith.BinInt.
 Local Open Scope Z.
+Require Import riscv.Utility.Utility.
 Local Open Scope alu_scope.
 
 (* Converted imports: *)
