src/Spec/VirtualMemory.v
@@ -1,0 +1,3 @@
+Require Import riscv.Spec.Machine.
+
+Notation translate := riscv.Spec.Machine.translate.
